Prove CWP wands for postcondition and contexts

theories/iris/language/cwp/def.v
@@ -13,6 +13,23 @@ Section def.
 
   Definition fvs_pred : Type := frame -> list value -> iProp Σ.
 
+  Definition label_wand (l1 l2 : label_spec) : iProp Σ :=
+    ⌜fst l1 = fst l2⌝ ∗ ∀ f vs, snd l1 f vs -∗ snd l2 f vs.
+
+  Definition label_ctx_wand (L1 L2 : list label_spec) : iProp Σ :=
+    ⌜length L1 <= length L2⌝ ∗ [∗ list] l1; l2 ∈ L1; take (length L1) L2, label_wand l1 l2.
+
+  Definition return_wand (r1 r2 : return_spec) : iProp Σ :=
+    ⌜fst r1 = fst r2⌝ ∗ ∀ vs, snd r1 vs -∗ snd r2 vs.
+
+  Definition return_ctx_wand (R1 R2 : option return_spec) : iProp Σ :=
+    match R1, R2 with
+    | Some _, None => False
+    | Some r1, Some r2 => return_wand r1 r2
+    | None, Some _ => True
+    | None, None => True
+    end%I.
+
   Definition fvs_combine (Φ : fvs_pred) (vs0 : list value) (f : frame) (vs : list value) : iProp Σ :=
     Φ f (vs0 ++ vs).
 
