theories/iris/logrel/compat_lemmas/shared.v
@@ -1162,9 +1162,9 @@ Section Fundamental_Shared.
         * cbn; eauto.
         * iApply (cwp_seq with "[Hframe Hrun]").
           {
-            iApply cwp_weak_take_labels.
+            iApply cwp_label_take.
             instantiate (2 := 0%nat).
-            iApply cwp_weak_no_return.
+            iApply cwp_return_none.
             iApply (cwp_mod2_test_1 with "[] [] [$] [$]"); eauto.
             iPureIntro.
             unfold Wasm_int.Int32.repr; simpl.
@@ -1183,9 +1183,9 @@ Section Fundamental_Shared.
           iApply (cwp_block with "[$] [$] [Hptr]").
           1, 2: done.
           iIntros "!> Hf Hrun".
-          iApply cwp_weak_take_labels.
+          iApply cwp_label_take.
           instantiate (1 := 0%nat).
-          iApply cwp_weak_no_return.
+          iApply cwp_return_none.
           iApply ("Hptr" with "[$] [$]").
       + done.
     - iDestruct "Hrep" as "(%l & -> & %rp & %Hrep & Hroot)".
@@ -1194,9 +1194,9 @@ Section Fundamental_Shared.
       inversion Hrep as [|? ? Hmod]; subst.
       iApply (cwp_seq with "[Hframe Hrun]").
       {
-        iApply cwp_weak_take_labels.
+        iApply cwp_label_take.
         instantiate (2 := 0%nat).
-        iApply cwp_weak_no_return.
+        iApply cwp_return_none.
         iApply (cwp_mod2_test_1_2 with "[] [] [$] [$]"); eauto.
         unfold Wasm_int.Int32.repr; simpl.
         rewrite Wasm_int.Int32.Z_mod_modulus_eq.
@@ -1229,9 +1229,9 @@ Section Fundamental_Shared.
         iIntros "!> Hf Hrun".
         cwp_chomp 4%nat.
         iApply (cwp_seq with "[Hf Hrun]").
-        * iApply cwp_weak_take_labels.
+        * iApply cwp_label_take.
           instantiate (2 := 0%nat).
-          iApply cwp_weak_no_return.
+          iApply cwp_return_none.
           iApply (cwp_mod4_sub3_test with "[//] [] [$] [$]"); eauto.
           iPureIntro.
           unfold Wasm_int.Int32.repr; simpl.
@@ -1253,9 +1253,9 @@ Section Fundamental_Shared.
           iApply (cwp_block with "[$] [$] [Hptr]").
           1, 2: done.
           iIntros "!> Hf Hrun".
-          iApply cwp_weak_take_labels.
+          iApply cwp_label_take.
           instantiate (1 := 0%nat).
-          iApply cwp_weak_no_return.
+          iApply cwp_return_none.
           iApply ("Hptr" with "[$] [$]").
       + simpl tag_address in Hlookup_f.
         cbn.
@@ -1266,9 +1266,9 @@ Section Fundamental_Shared.
         cwp_chomp 4%nat.
         rewrite take_0 drop_0.
         iApply (cwp_seq with "[Hf Hrun]").
-        * iApply cwp_weak_take_labels.
+        * iApply cwp_label_take.
           instantiate (2 := 0%nat).
-          iApply cwp_weak_no_return.
+          iApply cwp_return_none.
           iApply (cwp_mod4_sub1_test with "[//] [] [$] [$]").
           iPureIntro.
           unfold Wasm_int.Int32.repr; simpl.
@@ -1290,9 +1290,9 @@ Section Fundamental_Shared.
           iApply (cwp_block with "[$] [$] [Hptr]").
           1, 2: done.
           iIntros "!> Hf Hrun".
-          iApply cwp_weak_take_labels.
+          iApply cwp_label_take.
           instantiate (1 := 0%nat).
-          iApply cwp_weak_no_return.
+          iApply cwp_return_none.
           iApply ("Hptr" with "[$] [$]").
   Qed.
 
